feat (EpsilonNA): conversion of EpsilonNA into NA, with proof of correctness

Cslib/Computability/Automata/EpsilonNA.lean
@@ -6,9 +6,31 @@ Authors: Fabrizio Montesi
 
 import Cslib.Computability.Automata.NA
 
+/-! # Nondeterministic automata with ε-transitions. -/
+
+/-- A nondeterministic automaton with ε-transitions (`εNA`) is an `NA` with an `Option` symbol
+type. The special symbol ε is represented by the `Option.none` case.
+
+Internally, ε (`Option.none`) is treated as the `τ` label of the underlying transition system,
+allowing for reusing the definitions and results on saturated transitions of `LTS` to deal with
+ε-closure. -/
 structure εNA (State : Type _) (Symbol : Type _) extends NA State (Option Symbol)
 
+@[grind]
 private instance : HasTau (Option α) := ⟨.none⟩
+
+/-- The `ε`-closure of a set of states `S` is the set of states reachable by any state in `S`
+by performing only `ε`-transitions. We use `LTS.τClosure` since `ε` (`Option.none`) is an instance
+of `HasTau.τ`. -/
+abbrev εNA.εClosure (ena : εNA State Symbol) (S : Set State) := ena.τClosure S
+
+/-- Converts an `LTS` with Option labels into an `LTS` on the carried label type, by removing all
+ε-transitions. -/
+@[grind]
+private def LTS.noε (lts : LTS State (Option Label)) :
+  LTS State Label := {
+  Tr := fun s μ s' => lts.Tr s (some μ) s'
+}
 
 namespace εNA
 
@@ -16,7 +38,8 @@ namespace εNA
 from the start state. -/
 @[grind]
 def Accepts (ena : εNA State Symbol) (xs : List Symbol) :=
-  ∃ s ∈ ena.start, ∃ s' ∈ ena.accept, ena.saturate.MTr s xs s'
+  ∃ s ∈ ena.εClosure ena.start, ∃ s' ∈ ena.accept,
+  ena.saturate.MTr s (xs.map (some ·)) s'
 
 /-- The language of an εDA is the set of strings that it accepts. -/
 @[grind]
@@ -30,16 +53,66 @@ theorem accepts_mem_language (ena : εNA State Symbol) (xs : List Symbol) :
 
 section NA
 
+/-- Any εNA can be converted into an NA that does not use ε-transitions. -/
 @[grind]
 def toNAWithoutEpsilon (ena : εNA State Symbol) : NA State Symbol := {
-  start := ena.setImage ena.start HasTau.τ
+  start := ena.εClosure ena.start
   accept := ena.accept
-  Tr := fun s x s' => ena.saturate.Tr s (some x) s'
+  Tr := ena.saturate.noε.Tr
 }
 
--- theorem toNAWithoutEpsilon_language_eq {ena : εNA State Symbol} :
---   ena.toNAWithoutEpsilon.language = ena.language := by
---   grind
+@[grind]
+lemma LTS.noε_saturate_tr
+  {lts : LTS State (Option Label)} {h : μ = some μ'} :
+  lts.saturate.Tr s μ s' ↔ lts.saturate.noε.Tr s μ' s' := by
+  simp only [LTS.noε]
+  grind
+
+@[grind]
+lemma LTS.noε_saturate_mTr
+  {lts : LTS State (Option Label)} :
+  lts.saturate.MTr s (μs.map (some ·)) = lts.saturate.noε.MTr s μs := by
+  ext s'
+  induction μs generalizing s
+  case nil => grind
+  case cons μ μs ih =>
+    apply Iff.intro <;> intro h
+    case mp =>
+      simp only [LTS.noε]
+      cases h
+      rename_i sb htr hmtr
+      apply LTS.MTr.stepL (s1 := s) (s2 := sb) (s3 := s') <;> grind
+    case mpr =>
+      simp only [LTS.noε] at h
+      grind
+
+
+/-- Correctness of `toNAWithoutEpsilon`. -/
+@[grind]
+theorem toNAWithoutEpsilon_language_eq {ena : εNA State Symbol} :
+  ena.toNAWithoutEpsilon.language = ena.language := by
+  ext xs
+  apply Iff.intro
+  case mp =>
+    rw [← εNA.accepts_mem_language, ← NA.accepts_mem_language]
+    simp only [NA.Accepts, toNAWithoutEpsilon, Accepts, forall_exists_index, and_imp]
+    intro s hs s' hs' hmtr
+    exists s
+    apply And.intro hs
+    exists s'
+    apply And.intro hs'
+    rw [LTS.noε_saturate_mTr]
+    assumption
+  case mpr =>
+    rw [← εNA.accepts_mem_language, ← NA.accepts_mem_language]
+    simp only [NA.Accepts, toNAWithoutEpsilon, Accepts, forall_exists_index, and_imp]
+    intro s hs s' hs' hmtr
+    exists s
+    apply And.intro hs
+    exists s'
+    apply And.intro hs'
+    rw [← LTS.noε_saturate_mTr]
+    assumption
 
 end NA
 
